merge:xor,or,sub,and

theory/JITPer_aux.thy
@@ -90,6 +90,32 @@ definition per_jit_add_reg64_1 :: "bpf_ireg \<Rightarrow> bpf_ireg \<Rightarrow>
     Some (1, 0, x64_encode ins) 
 )"
 
+
+definition per_jit_sub_reg64_1 :: "bpf_ireg \<Rightarrow> bpf_ireg \<Rightarrow> (nat \<times> u64 \<times> x64_bin) option" where
+"per_jit_sub_reg64_1 dst src = (
+  let ins = Psubq_rr (bpf_to_x64_reg dst) (bpf_to_x64_reg src) in
+    Some (1, 0, x64_encode ins) 
+)"
+
+definition per_jit_or_reg64_1 :: "bpf_ireg \<Rightarrow> bpf_ireg \<Rightarrow> (nat \<times> u64 \<times> x64_bin) option" where
+"per_jit_or_reg64_1 dst src = (
+  let ins = Porq_rr (bpf_to_x64_reg dst) (bpf_to_x64_reg src) in
+    Some (1, 0, x64_encode ins) 
+)"
+
+definition per_jit_and_reg64_1 :: "bpf_ireg \<Rightarrow> bpf_ireg \<Rightarrow> (nat \<times> u64 \<times> x64_bin) option" where
+"per_jit_and_reg64_1 dst src = (
+  let ins = Pandq_rr (bpf_to_x64_reg dst) (bpf_to_x64_reg src) in
+    Some (1, 0, x64_encode ins) 
+)"
+
+definition per_jit_xor_reg64_1 :: "bpf_ireg \<Rightarrow> bpf_ireg \<Rightarrow> (nat \<times> u64 \<times> x64_bin) option" where
+"per_jit_xor_reg64_1 dst src = (
+  let ins = Pxorq_rr (bpf_to_x64_reg dst) (bpf_to_x64_reg src) in
+    Some (1, 0, x64_encode ins) 
+)"
+
+
 definition per_jit_exit :: "(nat \<times> u64 \<times> x64_bin) option" where
 "per_jit_exit = (
   let ins = Pret in
@@ -133,7 +159,7 @@ definition per_jit_jcc ::"condition \<Rightarrow> bpf_ireg \<Rightarrow> bpf_ire
 
 
 definition per_jit_call_reg :: "bpf_ireg \<Rightarrow> imm_ty \<Rightarrow> (nat \<times> u64 \<times> x64_bin) option" where
-  "per_jit_call_reg src imm = Some (1, 0, x64_encode (Pcall_i (ucast imm)))"
+  "per_jit_call_reg src imm = Some (1, ucast imm, x64_encode (Pcall_i 0))"
 
 definition per_jit_shift_lsh_reg64 :: "bpf_ireg \<Rightarrow> bpf_ireg \<Rightarrow> (nat \<times> u64 \<times> x64_bin) option" where
 "per_jit_shift_lsh_reg64 dst src = (
@@ -202,6 +228,10 @@ definition per_jit_ins ::" bpf_instruction \<Rightarrow> (nat \<times> u64 \<tim
 "per_jit_ins bins = (
   case bins of
   BPF_ALU64 BPF_ADD dst (SOReg src) \<Rightarrow> (per_jit_add_reg64_1 dst src) |
+  BPF_ALU64 BPF_SUB dst (SOReg src) \<Rightarrow> (per_jit_sub_reg64_1 dst src) |
+  BPF_ALU64 BPF_OR dst (SOReg src) \<Rightarrow> (per_jit_or_reg64_1 dst src) |
+  BPF_ALU64 BPF_AND dst (SOReg src) \<Rightarrow> (per_jit_and_reg64_1 dst src) |
+  BPF_ALU64 BPF_XOR dst (SOReg src) \<Rightarrow> (per_jit_xor_reg64_1 dst src) |
   BPF_EXIT \<Rightarrow> per_jit_exit |
   BPF_ALU64 BPF_MUL dst (SOReg src) \<Rightarrow> (per_jit_mul_reg64 dst src) |
   BPF_JUMP cond dst (SOReg src) off \<Rightarrow> per_jit_jcc cond dst src (scast off) |
@@ -396,6 +426,10 @@ lemma aux1:"length prog \<noteq> 0 \<and> unat pc < length prog \<and> unat pc \
   s = (SBPF_OK pc rs m ss) \<Longrightarrow> 
   s' = (SBPF_OK pc' rs' m' ss') \<Longrightarrow> 
   (\<exists> dst src. prog!(unat pc) = BPF_ALU64 BPF_ADD dst (SOReg src) \<or> 
+    prog!(unat pc) = BPF_ALU64 BPF_SUB dst (SOReg src) \<or>
+    prog!(unat pc) = BPF_ALU64 BPF_XOR dst (SOReg src) \<or>
+    prog!(unat pc) = BPF_ALU64 BPF_OR dst (SOReg src) \<or>
+    prog!(unat pc) = BPF_ALU64 BPF_AND dst (SOReg src) \<or>
     prog!(unat pc) = BPF_ALU64 BPF_MUL dst (SOReg src) \<or> 
     prog!(unat pc) = BPF_ALU64 BPF_LSH dst (SOReg src) \<or> 
     prog!(unat pc) = BPF_ALU64 BPF_RSH dst (SOReg src) \<or> 
@@ -416,7 +450,11 @@ lemma aux1:"length prog \<noteq> 0 \<and> unat pc < length prog \<and> unat pc \
        apply(cases x93, simp_all)
       apply(cases x93, simp_all)
      apply(cases x93, simp_all)
-    apply(cases x93, simp_all)
+          apply(cases x93, simp_all)
+      apply(cases x93, simp_all)
+        apply(cases x93, simp_all)
+      apply(cases x93, simp_all)
+      apply(cases x93, simp_all)
     done
   subgoal for x161 x162 x163 x164
     by(cases x163,simp_all)
@@ -609,9 +647,10 @@ lemma corr_pc_aux2:
   s =  SBPF_OK pc rs m ss \<Longrightarrow>
   s' = sbpf_step prog s \<Longrightarrow> s' = SBPF_OK pc' rs' m' ss' \<Longrightarrow> 
   (num,off,l) = x64_prog!(unat pc) \<Longrightarrow>
-  prog!(unat pc) \<in> {BPF_ALU64 BPF_ADD dst (SOReg src), BPF_ALU64 BPF_MUL dst (SOReg src), 
-  BPF_ALU64 BPF_LSH dst (SOReg src),BPF_ALU64 BPF_RSH dst (SOReg src), BPF_ALU64 BPF_ARSH dst (SOReg src),
-  BPF_LDX chk dst src d, BPF_ST chk dst (SOReg src) d} \<Longrightarrow>
+  prog!(unat pc) \<in> {BPF_ALU64 BPF_ADD dst (SOReg src), BPF_ALU64 BPF_SUB dst (SOReg src), 
+  BPF_ALU64 BPF_OR dst (SOReg src), BPF_ALU64 BPF_AND dst (SOReg src), BPF_ALU64 BPF_XOR dst (SOReg src),
+  BPF_ALU64 BPF_MUL dst (SOReg src), BPF_ALU64 BPF_LSH dst (SOReg src),BPF_ALU64 BPF_RSH dst (SOReg src), 
+  BPF_ALU64 BPF_ARSH dst (SOReg src), BPF_LDX chk dst src d, BPF_ST chk dst (SOReg src) d} \<Longrightarrow>
   pc' = pc + 1" 
 proof-
   assume assm0:"s' = sbpf_step prog s"  and
@@ -620,9 +659,10 @@ proof-
          assm3:"prog \<noteq> [] \<and> unat pc \<ge> 0 \<and> unat pc < length prog" and
          assm4:"s = SBPF_OK pc rs m ss" and
          assm5:"(num,off,l) = x64_prog!(unat pc)" and
-         assm6:" prog!(unat pc) \<in> {BPF_ALU64 BPF_ADD dst (SOReg src), BPF_ALU64 BPF_MUL dst (SOReg src),
-  BPF_ALU64 BPF_LSH dst (SOReg src),BPF_ALU64 BPF_RSH dst (SOReg src), BPF_ALU64 BPF_ARSH dst (SOReg src),
-  BPF_LDX chk dst src d, BPF_ST chk dst (SOReg src) d}"
+         assm6:" prog!(unat pc) \<in> {BPF_ALU64 BPF_ADD dst (SOReg src), BPF_ALU64 BPF_SUB dst (SOReg src), 
+  BPF_ALU64 BPF_OR dst (SOReg src), BPF_ALU64 BPF_AND dst (SOReg src), BPF_ALU64 BPF_XOR dst (SOReg src),
+  BPF_ALU64 BPF_MUL dst (SOReg src), BPF_ALU64 BPF_LSH dst (SOReg src),BPF_ALU64 BPF_RSH dst (SOReg src), 
+  BPF_ALU64 BPF_ARSH dst (SOReg src), BPF_LDX chk dst src d, BPF_ST chk dst (SOReg src) d}"
   have c1:"pc' = pc+1 " using assm6 assm0 assm1 
     apply(cases "prog!(unat pc)",simp_all)
        (*prefer 4 using assm4 assm3 apply simp*)
