theory/JITPer.thy
@@ -20,6 +20,7 @@ imports
   JITPer_exit JITPer_jump
   JITPer_load JITPer_shift
   JITPer_store JITPer_call JITPer_exit
+  JITPer_sub JITPer_and JITPer_xor JITPer_or
 
 begin
 
@@ -38,6 +39,10 @@ shows "\<exists> xst'. x64_sem1 1 x64_prog (pc,xst) = (pc',xst') \<and>
 proof-
   let "?bpf_ins" = "prog!(unat pc)"
   have b1:"(\<exists> dst src. prog!(unat pc) = BPF_ALU64 BPF_ADD dst (SOReg src) \<or> 
+    prog!(unat pc) = BPF_ALU64 BPF_SUB dst (SOReg src) \<or>
+    prog!(unat pc) = BPF_ALU64 BPF_XOR dst (SOReg src) \<or>
+    prog!(unat pc) = BPF_ALU64 BPF_OR dst (SOReg src) \<or>
+    prog!(unat pc) = BPF_ALU64 BPF_AND dst (SOReg src) \<or>
     prog!(unat pc) = BPF_ALU64 BPF_MUL dst (SOReg src) \<or> 
     prog!(unat pc) = BPF_ALU64 BPF_LSH dst (SOReg src) \<or> 
     prog!(unat pc) = BPF_ALU64 BPF_RSH dst (SOReg src) \<or> 
@@ -48,7 +53,11 @@ proof-
   (\<exists> src imm. prog!(unat pc) = BPF_CALL_IMM src imm) \<or>
   prog!(unat pc) = BPF_EXIT" using a0 a1 a2 a6 aux1 by fast
   obtain src dst x cond chk off imm where 
-    b2:"?bpf_ins = BPF_ALU64 BPF_ADD dst (SOReg src) \<or> 
+    b2:"?bpf_ins = BPF_ALU64 BPF_ADD dst (SOReg src) \<or>  
+        ?bpf_ins  = BPF_ALU64 BPF_SUB dst (SOReg src) \<or>
+        ?bpf_ins = BPF_ALU64 BPF_XOR dst (SOReg src) \<or>
+        ?bpf_ins = BPF_ALU64 BPF_OR dst (SOReg src) \<or>
+        ?bpf_ins = BPF_ALU64 BPF_AND dst (SOReg src) \<or>
         ?bpf_ins = BPF_ALU64 BPF_MUL dst (SOReg src) \<or> 
         ?bpf_ins = BPF_ALU64 BPF_LSH dst (SOReg src) \<or> 
         ?bpf_ins = BPF_ALU64 BPF_RSH dst (SOReg src) \<or> 
@@ -90,7 +99,11 @@ proof-
         ?bpf_ins = BPF_ST chk dst (SOReg src) off \<or> 
         ?bpf_ins = BPF_JUMP cond dst (SOReg src) x\<or>
         ?bpf_ins = BPF_CALL_IMM src imm \<or>
-        ?bpf_ins = BPF_EXIT" using False b2 by blast
+        ?bpf_ins = BPF_EXIT \<or>
+        ?bpf_ins  = BPF_ALU64 BPF_SUB dst (SOReg src) \<or>
+        ?bpf_ins = BPF_ALU64 BPF_XOR dst (SOReg src) \<or>
+        ?bpf_ins = BPF_ALU64 BPF_OR dst (SOReg src) \<or>
+        ?bpf_ins = BPF_ALU64 BPF_AND dst (SOReg src)" using False b2 by blast
       thus ?thesis 
       proof(cases "(?bpf_ins = BPF_JUMP cond dst (SOReg src) x)")
         case True
@@ -104,7 +117,11 @@ proof-
         ?bpf_ins = BPF_LDX chk dst src off \<or> 
         ?bpf_ins = BPF_ST chk dst (SOReg src) off\<or>
         ?bpf_ins = BPF_CALL_IMM src imm \<or>
-        ?bpf_ins = BPF_EXIT" using False c4 by simp
+        ?bpf_ins = BPF_EXIT \<or>
+        ?bpf_ins  = BPF_ALU64 BPF_SUB dst (SOReg src) \<or>
+        ?bpf_ins = BPF_ALU64 BPF_XOR dst (SOReg src) \<or>
+        ?bpf_ins = BPF_ALU64 BPF_OR dst (SOReg src) \<or>
+        ?bpf_ins = BPF_ALU64 BPF_AND dst (SOReg src)" using False c4 by simp
         thus ?thesis
         proof(cases "?bpf_ins = BPF_ALU64 BPF_ADD dst (SOReg src)")
           case True
@@ -117,7 +134,11 @@ proof-
           ?bpf_ins = BPF_LDX chk dst src off \<or> 
           ?bpf_ins = BPF_ST chk dst (SOReg src) off\<or>
           ?bpf_ins = BPF_CALL_IMM src imm \<or>
-          ?bpf_ins = BPF_EXIT" using False c5 by simp
+          ?bpf_ins = BPF_EXIT\<or>
+          ?bpf_ins  = BPF_ALU64 BPF_SUB dst (SOReg src) \<or>
+          ?bpf_ins = BPF_ALU64 BPF_XOR dst (SOReg src) \<or>
+          ?bpf_ins = BPF_ALU64 BPF_OR dst (SOReg src) \<or>
+          ?bpf_ins = BPF_ALU64 BPF_AND dst (SOReg src)" using False c5 by simp
           thus ?thesis
           proof(cases "?bpf_ins = BPF_ALU64 BPF_LSH dst (SOReg src)")
             case True
@@ -130,7 +151,11 @@ proof-
             ?bpf_ins = BPF_LDX chk dst src off \<or> 
             ?bpf_ins = BPF_ST chk dst (SOReg src) off\<or>
             ?bpf_ins = BPF_CALL_IMM src imm \<or>
-            ?bpf_ins = BPF_EXIT" using c6 False by simp
+            ?bpf_ins = BPF_EXIT\<or>
+            ?bpf_ins  = BPF_ALU64 BPF_SUB dst (SOReg src) \<or>
+            ?bpf_ins = BPF_ALU64 BPF_XOR dst (SOReg src) \<or>
+            ?bpf_ins = BPF_ALU64 BPF_OR dst (SOReg src) \<or>
+            ?bpf_ins = BPF_ALU64 BPF_AND dst (SOReg src)" using c6 False by simp
             then show ?thesis 
             proof(cases "?bpf_ins = BPF_ALU64 BPF_RSH dst (SOReg src)")
               case True
@@ -142,7 +167,11 @@ proof-
               ?bpf_ins = BPF_LDX chk dst src off \<or> 
               ?bpf_ins = BPF_ST chk dst (SOReg src) off\<or>
               ?bpf_ins = BPF_CALL_IMM src imm \<or>
-              ?bpf_ins = BPF_EXIT" using c7 False by simp
+              ?bpf_ins = BPF_EXIT \<or>
+              ?bpf_ins  = BPF_ALU64 BPF_SUB dst (SOReg src) \<or>
+              ?bpf_ins = BPF_ALU64 BPF_XOR dst (SOReg src) \<or>
+              ?bpf_ins = BPF_ALU64 BPF_OR dst (SOReg src) \<or>
+              ?bpf_ins = BPF_ALU64 BPF_AND dst (SOReg src)" using c7 False by simp
               then show ?thesis 
               proof(cases "?bpf_ins = BPF_ALU64 BPF_ARSH dst (SOReg src)")
                 case True
@@ -152,7 +181,11 @@ proof-
                 have c8:"?bpf_ins = BPF_LDX chk dst src off \<or> 
                 ?bpf_ins = BPF_ST chk dst (SOReg src) off\<or>
                 ?bpf_ins = BPF_CALL_IMM src imm \<or>
-                ?bpf_ins = BPF_EXIT" using c7 False by simp
+                ?bpf_ins = BPF_EXIT\<or>
+                ?bpf_ins  = BPF_ALU64 BPF_SUB dst (SOReg src) \<or>
+                ?bpf_ins = BPF_ALU64 BPF_XOR dst (SOReg src) \<or>
+                ?bpf_ins = BPF_ALU64 BPF_OR dst (SOReg src) \<or>
+                ?bpf_ins = BPF_ALU64 BPF_AND dst (SOReg src)" using c7 False by simp
                 then show ?thesis
                 proof(cases "?bpf_ins = BPF_LDX chk dst src off")
                   case True
@@ -162,7 +195,11 @@ proof-
                   case False
                   have c9:"?bpf_ins = BPF_ST chk dst (SOReg src) off\<or>
                   ?bpf_ins = BPF_CALL_IMM src imm \<or>
-                  ?bpf_ins = BPF_EXIT" using False c8 by simp
+                  ?bpf_ins = BPF_EXIT\<or>
+                  ?bpf_ins  = BPF_ALU64 BPF_SUB dst (SOReg src) \<or>
+                  ?bpf_ins = BPF_ALU64 BPF_XOR dst (SOReg src) \<or>
+                  ?bpf_ins = BPF_ALU64 BPF_OR dst (SOReg src) \<or>
+                  ?bpf_ins = BPF_ALU64 BPF_AND dst (SOReg src)" using False c8 by simp
                   then show ?thesis
                    proof(cases "?bpf_ins = BPF_ST chk dst (SOReg src) off")
                      case True
@@ -171,15 +208,64 @@ proof-
                    next
                      case False
                      have c10:"?bpf_ins = BPF_CALL_IMM src imm \<or>
-                     ?bpf_ins = BPF_EXIT" using False c9 by simp
+                     ?bpf_ins = BPF_EXIT\<or>
+                     ?bpf_ins  = BPF_ALU64 BPF_SUB dst (SOReg src) \<or>
+                     ?bpf_ins = BPF_ALU64 BPF_XOR dst (SOReg src) \<or>
+                     ?bpf_ins = BPF_ALU64 BPF_OR dst (SOReg src) \<or>
+                     ?bpf_ins = BPF_ALU64 BPF_AND dst (SOReg src)" using False c9 by simp
                      then show ?thesis
                       proof(cases "?bpf_ins = BPF_CALL_IMM src imm")
                         case True
                         then show ?thesis using call_imm_one_step a0 a1 a2 a3 a4 a5 a6 True by simp
                       next
                         case False
-                        have "?bpf_ins = BPF_EXIT" using c10 False by simp
-                        then show ?thesis using exit_one_step a0 a1 a2 a3 a4 a5 a6 False by blast
+                        have c11:"?bpf_ins = BPF_EXIT\<or>
+                              ?bpf_ins  = BPF_ALU64 BPF_SUB dst (SOReg src) \<or>
+                              ?bpf_ins = BPF_ALU64 BPF_XOR dst (SOReg src) \<or>
+                              ?bpf_ins = BPF_ALU64 BPF_OR dst (SOReg src) \<or>
+                              ?bpf_ins = BPF_ALU64 BPF_AND dst (SOReg src)" using c10 False by simp
+
+                        then show ?thesis 
+                        proof(cases "?bpf_ins = BPF_EXIT")
+                          case True
+                          then show ?thesis using exit_one_step a0 a1 a2 a3 a4 a5 a6 True by blast
+                        next
+                          case False
+                          have c12:"?bpf_ins  = BPF_ALU64 BPF_SUB dst (SOReg src) \<or>
+                              ?bpf_ins = BPF_ALU64 BPF_XOR dst (SOReg src) \<or>
+                              ?bpf_ins = BPF_ALU64 BPF_OR dst (SOReg src) \<or>
+                              ?bpf_ins = BPF_ALU64 BPF_AND dst (SOReg src)" using c11 False by simp
+                          then show ?thesis 
+                          proof(cases "?bpf_ins  = BPF_ALU64 BPF_SUB dst (SOReg src)")
+                            case True
+                            then show ?thesis using subq_one_step a0 a1 a2 a3 a4 a5 a6 True by blast
+                          next
+                            case False
+                              have c13:"?bpf_ins = BPF_ALU64 BPF_XOR dst (SOReg src) \<or>
+                              ?bpf_ins = BPF_ALU64 BPF_OR dst (SOReg src) \<or>
+                              ?bpf_ins = BPF_ALU64 BPF_AND dst (SOReg src)" using c12 False by simp
+                            then show ?thesis 
+                            proof(cases "?bpf_ins = BPF_ALU64 BPF_XOR dst (SOReg src)")
+                              case True
+                              then show ?thesis using xorq_one_step a0 a1 a2 a3 a4 a5 a6 True by blast
+                            next
+                              case False
+                              have c14:"?bpf_ins = BPF_ALU64 BPF_OR dst (SOReg src) \<or>
+                              ?bpf_ins = BPF_ALU64 BPF_AND dst (SOReg src)" using c13 False by simp
+                              then show ?thesis 
+                              proof(cases "?bpf_ins = BPF_ALU64 BPF_OR dst (SOReg src)")
+                                case True
+                                then show ?thesis using orq_one_step a0 a1 a2 a3 a4 a5 a6 True by blast
+                              next
+                                case False
+                                have "?bpf_ins = BPF_ALU64 BPF_AND dst (SOReg src)" using c14 False by simp
+                                then show ?thesis using andq_one_step a0 a1 a2 a3 a4 a5 a6 False by blast
+                                qed
+                              qed
+                            qed
+                          qed
+                        qed
+                          
                       qed
                     qed
                 qed
