theory/JITPer_or.thy
@@ -1,0 +1,139 @@
+theory JITPer_or
+imports
+  Main
+  rBPFCommType rBPFSyntax rBPFSem
+  x64Syntax x64Semantics x64Assembler
+  JITPer_aux
+
+begin
+
+lemma orq_one_step_match_reg:
+  " (SBPF_OK pc' rs' m' ss') = sbpf_step prog (SBPF_OK pc rs m ss) \<Longrightarrow>
+    xst = (Next xpc xrs xm xss) \<Longrightarrow>
+    match_state (SBPF_OK pc rs m ss) (pc,xst) \<Longrightarrow>
+    prog \<noteq> [] \<and> unat pc < length prog \<and> unat pc \<ge> 0 \<Longrightarrow>
+    prog!(unat pc) = BPF_ALU64 BPF_OR dst (SOReg src) \<Longrightarrow>
+    match_reg rs' (xrs(IR (bpf_to_x64_reg dst) := or (xrs (IR (bpf_to_x64_reg dst))) (xrs (IR (bpf_to_x64_reg src)))))"
+  apply (simp add: match_state_def match_reg_def eval_alu_def eval_reg_def)
+  done
+
+lemma orq_one_step_match_mem:
+  " (SBPF_OK pc' rs' m' ss') = sbpf_step prog (SBPF_OK pc rs m ss) \<Longrightarrow>
+    xst = (Next xpc xrs xm xss) \<Longrightarrow>
+    match_state (SBPF_OK pc rs m ss) (pc,xst) \<Longrightarrow>
+    prog \<noteq> [] \<and> unat pc < length prog \<and> unat pc \<ge> 0 \<Longrightarrow>
+    prog!(unat pc) = BPF_ALU64 BPF_OR dst (SOReg src) \<Longrightarrow>
+   x64_encode (Porq_rr (bpf_to_x64_reg dst) (bpf_to_x64_reg src)) ! Suc (0::nat) \<noteq> (57::8 word) \<Longrightarrow> match_mem m' xm"
+  apply (simp add: match_state_def match_mem_def eval_alu_def eval_reg_def)
+  done
+  
+lemma orq_one_step_match_stack:
+  " (SBPF_OK pc' rs' m' ss') = sbpf_step prog (SBPF_OK pc rs m ss) \<Longrightarrow>
+    xst = (Next xpc xrs xm xss) \<Longrightarrow>
+    match_state (SBPF_OK pc rs m ss) (pc,xst) \<Longrightarrow>
+    prog \<noteq> [] \<and> unat pc < length prog \<and> unat pc \<ge> 0 \<Longrightarrow>
+    prog!(unat pc) = BPF_ALU64 BPF_OR dst (SOReg src) \<Longrightarrow>
+    x64_encode (Porq_rr (bpf_to_x64_reg dst) (bpf_to_x64_reg src)) ! Suc (0::nat) \<noteq> (57::8 word) \<Longrightarrow>
+    match_stack (xrs(IR (bpf_to_x64_reg dst) := or (xrs (IR (bpf_to_x64_reg dst))) (xrs (IR (bpf_to_x64_reg src)))))"
+  apply (simp add: match_state_def match_stack_def eval_alu_def eval_reg_def)
+  using reg_rsp_consist by blast 
+
+lemma orq_one_step_match_stack2:
+  "(SBPF_OK pc' rs' m' ss') = sbpf_step prog (SBPF_OK pc rs m ss) \<Longrightarrow>
+    prog \<noteq> [] \<and> unat pc < length prog \<and> unat pc \<ge> 0 \<Longrightarrow>
+    prog!(unat pc) = BPF_ALU64 BPF_OR dst (SOReg src) \<Longrightarrow>
+    xst = (Next xpc xrs xm xss) \<Longrightarrow>
+    match_state (SBPF_OK pc rs m ss) (pc,xst) \<Longrightarrow> xss=ss'"
+  apply(cases"prog!(unat pc)",simp_all)
+  subgoal for x91 
+    apply(cases "eval_alu BPF_OR dst (SOReg src) rs",simp_all)
+    apply(unfold match_state_def,simp_all)
+    done
+  done
+
+lemma orq_one_step:
+ assumes a0:"s' = sbpf_step prog s" and
+  a1:"s = (SBPF_OK pc rs m ss)" and
+  a2:"s' = (SBPF_OK pc' rs' m' ss')" and
+  a3:"xst = (Next xpc xrs xm xss)" and
+  a4:"match_state s (pc,xst)" and
+  a5:"jitper prog = Some x64_prog" and                      
+  a6:"prog \<noteq> [] \<and> unat pc < length prog \<and> unat pc \<ge> 0" and
+  a8:"prog!(unat pc) = BPF_ALU64 BPF_OR dst (SOReg src)" 
+shows "\<exists> xst'. x64_sem1 1 x64_prog (pc,xst) = (pc',xst') \<and> 
+  match_state s' (pc',xst')"
+  apply simp
+
+(* 1. as BPF_OR generates a single list of jited x64 assembly, so we only need one step  *)
+  apply(subgoal_tac "\<exists>xst'::outcome. one_step x64_prog (pc, xst) = (pc', xst') \<and> match_state s' (pc', xst')")
+  subgoal
+    by auto
+  subgoal
+    apply (unfold one_step_def Let_def)
+(* 2. according to the code structure of JITPer, removing the first case statement *)
+    apply(subgoal_tac "x64_prog ! unat (fst (pc, xst)) = the (per_jit_or_reg64_1 dst src)")
+     prefer 2
+    subgoal
+      using a5 a6 a8 aux5 per_jit_ins_def by fastforce
+    subgoal
+      apply (subgoal_tac "the (per_jit_or_reg64_1 dst src) = (1, 0, x64_encode (Porq_rr (bpf_to_x64_reg dst) (bpf_to_x64_reg src)))")
+       prefer 2
+      subgoal by (simp add: per_jit_or_reg64_1_def)
+      apply (subgoal_tac "(x64_encode (Porq_rr (bpf_to_x64_reg dst) (bpf_to_x64_reg src)))!1 \<noteq> 0x39 \<and> 
+              (x64_encode (Porq_rr (bpf_to_x64_reg dst) (bpf_to_x64_reg src)))!0 \<noteq> 0xc3\<and> 
+              (x64_encode (Porq_rr (bpf_to_x64_reg dst) (bpf_to_x64_reg src)))!0 \<noteq> 0xe8 ")
+       prefer 2
+      subgoal apply(unfold x64_encode_def) 
+        apply(cases "Porq_rr (bpf_to_x64_reg dst) (bpf_to_x64_reg src)",simp_all) 
+        subgoal for x11 apply(unfold per_jit_or_reg64_1_def construct_rex_to_u8_def bitfield_insert_u8_def Let_def u8_of_bool_def,simp_all)
+          apply(cases "and (u8_of_ireg (bpf_to_x64_reg src)) (8::8 word) \<noteq> (0::8 word)",simp_all)
+           apply(cases "and (u8_of_ireg x11) (8::8 word) \<noteq> (0::8 word)",simp_all)
+          apply(cases "and (u8_of_ireg x11) (8::8 word) \<noteq> (0::8 word)",simp_all)
+           done
+         done
+      subgoal
+        unfolding a3
+        apply simp
+        apply (erule subst)
+        apply (erule subst)
+(* 3. here we get a simplified version, next step is to remove another case statement *)
+        apply (subgoal_tac "x64_decode 0 (x64_encode (Porq_rr (bpf_to_x64_reg dst) (bpf_to_x64_reg src))) = Some (3, Porq_rr (bpf_to_x64_reg dst) (bpf_to_x64_reg src))")
+         prefer 2
+        subgoal
+          apply (rule_tac l_bin = "(x64_encode (Porq_rr (bpf_to_x64_reg dst) (bpf_to_x64_reg src)))" in x64_encode_decode_consistency)
+          subgoal by (rule list_in_list_prop)
+          subgoal by simp
+          subgoal using x64_encode_def
+            by fastforce
+          done
+        subgoal
+          apply simp
+          apply (erule subst)
+
+(* 4. now we get exec_instr (one step of x64 add assembly), we prove the \<and>, first left, then right *)
+        apply (simp add: exec_instr_def)
+        apply (rule conjI)
+        subgoal
+          by (metis a0 a1 a2 a5 a6 a8 corr_pc_aux2 insert_iff prod_cases3)
+
+        unfolding a1 a2
+        apply (simp add: match_state_def)
+        apply (rule conjI)
+
+(* 4.1  match_reg *)
+        subgoal using orq_one_step_match_reg a0 a1 a2 a3 a4 a6 a8
+          by simp
+
+        apply (rule conjI)
+(* 4.2  match_mem *)
+        subgoal using orq_one_step_match_mem a0 a1 a2 a3 a4 a6 a8 by simp
+(* 4.2  match_stack *)
+        subgoal using orq_one_step_match_stack a0 a1 a2 a3 a4 a6 a8 apply simp
+          using orq_one_step_match_stack2 a0 a1 a2 a3 a4 a6 a8 by (metis (no_types, lifting)) 
+        done
+        done
+      done
+    done       
+  done      
+
+end
